Refactor predicates on register file

src/opt/Compatibility.v
@@ -24,142 +24,6 @@ Set Implicit Arguments.
 
 Definition SIM_REGS := forall (rs_src rs_tgt:RegFile.t), Prop.
 
-Definition eq_except (regs:RegSet.t) (rs_src rs_tgt:RegFile.t): Prop :=
-  forall reg (REG: ~ RegSet.mem reg regs), rs_src reg = rs_tgt reg.
-
-Lemma eq_except_nil rs_src rs_tgt:
-  rs_src = rs_tgt <-> eq_except RegSet.empty rs_src rs_tgt.
-Proof.
-  econs; i; subst; auto.
-  - econs.
-  - extensionality reg. apply H. auto.
-Qed.
-
-Lemma eq_except_mon regs1 regs2
-      (SUB: RegSet.Subset regs1 regs2):
-  eq_except regs1 <2= eq_except regs2.
-Proof.
-  ii. specialize (PR reg). apply PR. contradict REG.
-  apply IdentSet.Facts.mem_iff. apply SUB.
-  apply IdentSet.Facts.mem_iff. auto.
-Qed.
-
-Lemma eq_except_singleton r v rs:
-  eq_except (RegSet.singleton r) (RegFun.add r v rs) rs.
-Proof.
-  ii. unfold RegFun.add, RegFun.find.
-  destruct (Reg.eq_dec reg r); auto. subst.
-  contradict REG. rewrite LocSet.Facts.singleton_b.
-  unfold LocSet.Facts.eqb. destruct (Reg.eq_dec r r); congruence.
-Qed.
-
-Lemma eq_except_value
-      rs_src rs_tgt regs v
-      (REGS: RegSet.disjoint regs (Value.regs_of v))
-      (RS: eq_except regs rs_src rs_tgt):
-  RegFile.eval_value rs_src v = RegFile.eval_value rs_tgt v.
-Proof.
-  destruct v; auto. ss. apply RS. ii.
-  eapply REGS; eauto.
-  apply RegSet.Facts.mem_iff.
-  apply RegSet.Facts.singleton_iff. auto.
-Qed.
-
-Lemma eq_except_value_list
-      rs_src rs_tgt regs vl
-      (REGS: RegSet.disjoint regs (Value.regs_of_list vl))
-      (RS: eq_except regs rs_src rs_tgt):
-  map (RegFile.eval_value rs_src) vl = map (RegFile.eval_value rs_tgt) vl.
-Proof.
-  revert REGS. induction vl; ss. i. f_equal.
-  - eapply eq_except_value; eauto.
-    ii. eapply REGS; eauto.
-    destruct a; ss.
-    apply RegSet.Facts.mem_iff in RHS.
-    apply RegSet.Facts.mem_iff.
-    apply RegSet.singleton_spec in RHS. subst.
-    apply RegSet.add_spec. auto.
-  - apply IHvl.
-    ii. eapply REGS; eauto.
-    destruct a; ss.
-    apply RegSet.Facts.mem_iff in RHS.
-    apply RegSet.Facts.mem_iff.
-    apply RegSet.add_spec. auto.
-Qed.
-
-Lemma eq_except_expr
-      rs_src rs_tgt regs e
-      (REGS: RegSet.disjoint regs (Instr.regs_of_expr e))
-      (RS: eq_except regs rs_src rs_tgt):
-  RegFile.eval_expr rs_src e = RegFile.eval_expr rs_tgt e.
-Proof.
-  destruct e; ss.
-  - erewrite eq_except_value; eauto.
-  - erewrite eq_except_value; eauto.
-  - erewrite (eq_except_value op1); eauto.
-    + erewrite (eq_except_value op2); eauto.
-      ii. eapply REGS; eauto.
-      apply RegSet.Facts.mem_iff in RHS.
-      apply RegSet.Facts.mem_iff.
-      apply RegSet.union_spec. auto.
-    + ii. eapply REGS; eauto.
-      apply RegSet.Facts.mem_iff in RHS.
-      apply RegSet.Facts.mem_iff.
-      apply RegSet.union_spec. auto.
-Qed.
-
-Lemma eq_except_instr
-      rs1_src rs1_tgt rs2_tgt regs instr e
-      (TGT: RegFile.eval_instr rs1_tgt instr e rs2_tgt)
-      (REGS: RegSet.disjoint regs (Instr.regs_of instr))
-      (RS: eq_except regs rs1_src rs1_tgt):
-  exists rs2_src,
-    <<SRC: RegFile.eval_instr rs1_src instr e rs2_src>> /\
-    <<RS: eq_except regs rs2_src rs2_tgt>>.
-Proof.
-  inv TGT; ss.
-  - eexists. splits; [econs|].
-    ii. apply RS. auto.
-  - eexists. splits; [econs|].
-    ii. generalize (RS reg). i.
-    unfold RegFun.add, RegFun.find.
-    destruct (Reg.eq_dec reg lhs); auto.
-    subst. eapply eq_except_expr; eauto.
-    ii. eapply REGS; eauto.
-    apply RegSet.Facts.mem_iff in RHS.
-    apply RegSet.Facts.mem_iff.
-    apply RegSet.add_spec. auto.
-  - eexists. splits; [econs|].
-    ii. specialize (RS reg).
-    unfold RegFun.add, RegFun.find.
-    destruct (Reg.eq_dec reg lhs); auto.
-  - erewrite <- eq_except_value; eauto.
-    eexists. splits; [econs|].
-    ii. specialize (RS reg).
-    unfold RegFun.add, RegFun.find.
-    destruct (Reg.eq_dec reg lhs); auto.
-  - erewrite <- eq_except_value; eauto.
-    + eexists. splits; [econs|].
-      ii. specialize (RS reg).
-      unfold RegFun.add, RegFun.find.
-      destruct (Reg.eq_dec reg lhs); auto.
-    + ii. eapply REGS; eauto.
-      apply RegSet.Facts.mem_iff in RHS.
-      apply RegSet.Facts.mem_iff.
-      apply RegSet.add_spec. auto.
-  - eexists. splits; [econs|]. auto.
-  - erewrite <- eq_except_value_list; eauto.
-    + eexists. splits; [econs|].
-      ii. specialize (RS reg).
-      unfold RegFun.add, RegFun.find.
-      destruct (Reg.eq_dec reg lhs); auto.
-    + ii. eapply REGS; eauto.
-      apply RegSet.Facts.mem_iff in RHS.
-      apply RegSet.Facts.mem_iff.
-      apply RegSet.add_spec. auto.
-Qed.
-
-
 Inductive sim_terminal
           (sim_regs:SIM_REGS)
           (th_src th_tgt:Thread.t lang): Prop :=
@@ -385,10 +249,10 @@ Inductive ctx (sim_thread:SIM_THREAD lang lang): SIM_THREAD lang lang :=
     commit_src commit_tgt
     promise
     (REGS: RegSet.disjoint regs (Instr.regs_of instr))
-    (RS: eq_except regs rs_src rs_tgt)
+    (RS: RegFile.eq_except regs rs_src rs_tgt)
     (COMMIT: Commit.le commit_src commit_tgt):
     ctx sim_thread
-        (sim_terminal (eq_except regs))
+        (sim_terminal (RegFile.eq_except regs))
         (Thread.mk lang (State.mk rs_src [Stmt.instr instr]) commit_src promise) mem_k_src
         (Thread.mk lang (State.mk rs_tgt [Stmt.instr instr]) commit_tgt promise) mem_k_tgt
 | ctx_seq
@@ -495,7 +359,7 @@ Proof.
     { ss. subst. eexists _, _. splits; eauto. }
     inv STEP_TGT; ss.
     + inv STEP; ss; try inv STATE.
-      * exploit eq_except_instr; eauto. i. des.
+      * exploit RegFile.eq_except_instr; eauto. i. des.
         generalize GET. intro X. apply MEMORY in X.
         eexists _, _, _, _. splits; eauto.
         { econs 1. econs 1; eauto. econs; eauto.
@@ -503,7 +367,7 @@ Proof.
           admit. (* commit wf *)
         }
         { apply rclo5_step. apply ctx_nil; auto. reflexivity. }
-      * exploit eq_except_instr; eauto. i. des.
+      * exploit RegFile.eq_except_instr; eauto. i. des.
         exploit MemInv.write; try apply MEMORY0; eauto.
         { apply WF_SRC. }
         { apply WF_TGT. }
@@ -515,7 +379,7 @@ Proof.
           admit. (* commit wf *)
         }
         { apply rclo5_step. apply ctx_nil; auto. reflexivity. }
-      * exploit eq_except_instr; eauto. i. des.
+      * exploit RegFile.eq_except_instr; eauto. i. des.
         generalize GET. intro X. apply MEMORY in X.
         exploit MemInv.write; try apply MEMORY0; eauto.
         { apply WF_SRC. }
@@ -528,14 +392,14 @@ Proof.
           admit. (* commit wf *)
         }
         { apply rclo5_step. apply ctx_nil; auto. reflexivity. }
-      * exploit eq_except_instr; eauto. i. des.
+      * exploit RegFile.eq_except_instr; eauto. i. des.
         eexists _, _, _, _. splits; eauto.
         { econs 1. econs 4; eauto. econs; eauto.
           s. eapply Commit.fence_mon; eauto.
           admit. (* commit wf *)
         }
         { apply rclo5_step. apply ctx_nil; auto. reflexivity. }
-      * exploit eq_except_instr; eauto. i. des.
+      * exploit RegFile.eq_except_instr; eauto. i. des.
         eexists _, _, _, _. splits; eauto.
         { econs 1. econs 5; eauto. econs; eauto.
           admit. (* commit wf *)
@@ -553,7 +417,7 @@ Proof.
         }
         { apply rclo5_step. apply ctx_instr; auto. }
     + inv STATE.
-      exploit eq_except_instr; eauto. i. des.
+      exploit RegFile.eq_except_instr; eauto. i. des.
       eexists _, _, _, _. splits; eauto.
       * econs 2; eauto. econs; eauto.
         admit. (* commit wf *)
@@ -720,7 +584,7 @@ Qed.
 Lemma sim_stmts_instr
       instr regs
       (REGS: RegSet.disjoint regs (Instr.regs_of instr)):
-  sim_stmts (eq_except regs) [Stmt.instr instr] [Stmt.instr instr] (eq_except regs).
+  sim_stmts (RegFile.eq_except regs) [Stmt.instr instr] [Stmt.instr instr] (RegFile.eq_except regs).
 Proof.
   ii. pupto5_init. pupto5 ctx_weak_respectful.
 Qed.
